Repair broken theory

Locally_Nameless_Lambda_Calculus/First_Order_to_Higher_Order_Terms.thy
@@ -1,29 +1,8 @@
 theory First_Order_to_Higher_Order_Terms
   imports
     "First_Order_Terms.Term"
-    LN_HO_Term
+    LN_Lambda_Term
 begin
-
-primrec foterm_to_hoterm :: "('f, 'v) Term.term \<Rightarrow> ('f, 'v) LN_HO_Term.term"  where
-  "foterm_to_hoterm (Term.Var x) = Free x" |
-  "foterm_to_hoterm (Term.Fun f ts) = foldl App (Const f) (map foterm_to_hoterm ts)"
-
-lemma
-  fixes z :: "('f, 'v) term"
-  assumes "\<And>x y. App x y \<noteq> z"
-  shows "inj (foldl App z)"
-proof (rule injI)
-  fix xs ys :: "('f, 'v) term list"
-  assume "foldl App z xs = foldl App z ys"
-  thus "xs = ys"
-    using assms
-  proof (induction xs ys arbitrary: z rule: List.rev_induct2)
-    case (3 y ys)
-    hence False
-      by (metis foldl_Cons foldl_Nil foldl_append)
-    thus ?case ..
-  qed simp_all
-qed
 
 lemma foldl_def_eq_def_iff_list_eq_nil:
   assumes "\<And>x y. f x y \<noteq> e"
@@ -39,10 +18,31 @@ next
     by (metis foldl_Cons foldl_Nil foldl_append rev_exhaust)
 qed
 
+primrec foterm_to_hoterm :: "('c, 'f) Term.term \<Rightarrow> ('\<tau>, 'c, 'f) LN_Lambda_Term.preterm"  where
+  "foterm_to_hoterm (Term.Var x) = Free x" |
+  "foterm_to_hoterm (Term.Fun f ts) = foldl App (Const f [] []) (map foterm_to_hoterm ts)"
+
+lemma
+  fixes z :: "('\<tau>, 'c, 'f) LN_Lambda_Term.preterm"
+  assumes "\<And>x y. App x y \<noteq> z"
+  shows "inj (foldl App z)"
+proof (rule injI)
+  fix xs ys :: "('\<tau>, 'c, 'f) LN_Lambda_Term.preterm list"
+  assume "foldl App z xs = foldl App z ys"
+  thus "xs = ys"
+    using assms
+  proof (induction xs ys arbitrary: z rule: List.rev_induct2)
+    case (3 y ys)
+    hence False
+      by (metis foldl_Cons foldl_Nil foldl_append)
+    thus ?case ..
+  qed simp_all
+qed
+
 lemma foterm_to_hoterm_Fun_eq_Const_or_App:
-  fixes f args
+  fixes f :: "'c" and args :: "('c, 'f) Term.term list"
   shows
-    "foterm_to_hoterm (Term.Fun f args) = Const f \<or>
+    "foterm_to_hoterm (Term.Fun f args) = Const f [] [] \<or>
     (\<exists>t\<^sub>1 t\<^sub>2. foterm_to_hoterm (Term.Fun f args) = App t\<^sub>1 t\<^sub>2)"
 proof (induction args)
   case Nil
@@ -52,38 +52,40 @@ next
   case (Cons arg args)
   then show ?case (is "?CONS \<or> ?APP")
   proof (elim disjE exE)
-    assume "foterm_to_hoterm (Term.Fun f args) = Const f"
+    assume "foterm_to_hoterm (Term.Fun f args) = Const f [] []"
     then have "args = []"
       by (simp add: foldl_def_eq_def_iff_list_eq_nil)
     then have "?APP"
       by simp
     then show ?thesis ..
   next
-    fix t\<^sub>1 t\<^sub>2
+    fix t\<^sub>1 t\<^sub>2 :: "('\<tau>, 'c, 'f) LN_Lambda_Term.preterm"
     have "foterm_to_hoterm (Term.Fun f (arg # args)) =
-      foldl App (Const f) (foterm_to_hoterm arg # map foterm_to_hoterm args)"
+      foldl App (Const f [] []) (foterm_to_hoterm arg # map foterm_to_hoterm args)"
       unfolding foterm_to_hoterm.simps
       using foldl_append[of _ _ "[_]", unfolded append_Cons append_Nil]
       by simp
-    also have "\<dots> = foldl App (App (Const f) (foterm_to_hoterm arg)) (map foterm_to_hoterm args)"
+    also have "\<dots> = foldl App (App (Const f [] []) (foterm_to_hoterm arg)) (map foterm_to_hoterm args)"
       by simp
     finally have "foterm_to_hoterm (Term.Fun f (arg # args)) =
-      foldl App (App (Const f) (foterm_to_hoterm arg)) (map foterm_to_hoterm args)" .
+      foldl App (App (Const f [] []) (foterm_to_hoterm arg)) (map foterm_to_hoterm args)" .
     moreover assume "foterm_to_hoterm (Term.Fun f args) = App t\<^sub>1 t\<^sub>2"
     ultimately have "?APP"
-      by (metis (no_types, opaque_lifting)
-          foldl_Cons foldl_Nil foldl_append foldl_def_eq_def_iff_list_eq_nil
-          foterm_to_hoterm.simps(2) rev_exhaust)
+      by (metis (no_types, opaque_lifting) foldl_Cons
+          foldl_Nil foldl_append list.distinct(1)
+          rev_exhaust)
     then show ?thesis ..
   qed
 qed
 
-lemma inj_on_foterm_to_hoterm: "inj_on foterm_to_hoterm A"
+lemma inj_on_foterm_to_hoterm:
+  fixes A :: "('c, 'f) Term.term set"
+  shows "inj_on foterm_to_hoterm A"
 proof (rule inj_onI)
-  fix s and t :: "('f, 'v) Term.term"
-  assume "foterm_to_hoterm s = foterm_to_hoterm t"
+  fix s and t :: "('c, 'f) Term.term"
+  assume "foterm_to_hoterm s = (foterm_to_hoterm t :: ('\<tau>, 'c, 'f) preterm)"
   then show "s = t"
-  proof (induction s arbitrary: t)
+  proof (induction s arbitrary: t rule: Term.term.induct)
     case Var\<^sub>s: (Var x\<^sub>s)
     show ?case
     proof (cases t)
@@ -92,10 +94,11 @@ proof (rule inj_onI)
         using Var\<^sub>s by simp
     next
       case (Fun f\<^sub>t args\<^sub>t)
-      then show ?thesis
+      then have False
         using Var\<^sub>s foterm_to_hoterm_Fun_eq_Const_or_App
-        by (metis LN_HO_Term.term.distinct(1,11)
-            foterm_to_hoterm.simps(1))
+        by (metis foterm_to_hoterm.simps(1)
+            preterm.distinct(1,11))
+      then show ?thesis ..
     qed
   next
     case Fun\<^sub>s: (Fun f\<^sub>s args\<^sub>s)
@@ -104,26 +107,26 @@ proof (rule inj_onI)
       case (Var x\<^sub>t)
       then have False
         using Fun\<^sub>s
-        by (metis LN_HO_Term.term.distinct(1)
-            LN_HO_Term.term.simps(17) foterm_to_hoterm.simps(1)
-            foterm_to_hoterm_Fun_eq_Const_or_App)
+        by (metis foterm_to_hoterm.simps(1)
+            foterm_to_hoterm_Fun_eq_Const_or_App
+            preterm.distinct(1,11))
       then show ?thesis ..
     next
       case Fun\<^sub>t: (Fun f\<^sub>t args\<^sub>t)
-      have "foterm_to_hoterm (Term.Fun f\<^sub>s args\<^sub>s) = foterm_to_hoterm (Term.Fun f\<^sub>t args\<^sub>t)"
-        unfolding Fun\<^sub>s Fun\<^sub>t ..
+      have "foterm_to_hoterm (Term.Fun f\<^sub>s args\<^sub>s) = (foterm_to_hoterm (Term.Fun f\<^sub>t args\<^sub>t) :: ('\<tau>, 'c, 'f) preterm)"
+        unfolding Fun\<^sub>s.prems Fun\<^sub>t ..
 
-      hence "foldl App (Const f\<^sub>s) (map foterm_to_hoterm args\<^sub>s) =
-        foldl App (Const f\<^sub>t) (map foterm_to_hoterm args\<^sub>t)"
+      hence "foldl App (Const f\<^sub>s [] []) (map foterm_to_hoterm args\<^sub>s) =
+        (foldl App (Const f\<^sub>t [] []) (map foterm_to_hoterm args\<^sub>t) :: ('\<tau>, 'c, 'f) preterm)"
         by simp
 
-      hence "f\<^sub>s = f\<^sub>t" and "map foterm_to_hoterm args\<^sub>s = map foterm_to_hoterm args\<^sub>t"
+      hence "f\<^sub>s = f\<^sub>t" and "map foterm_to_hoterm args\<^sub>s = (map foterm_to_hoterm args\<^sub>t :: ('\<tau>, 'c, 'f) preterm list)"
         by simp_all
 
       hence "args\<^sub>s = args\<^sub>t"
       proof (elim list.inj_map_strong[rotated])
         show "\<And>z za. z \<in> set args\<^sub>s \<Longrightarrow> za \<in> set args\<^sub>t \<Longrightarrow>
-          foterm_to_hoterm z = foterm_to_hoterm za \<Longrightarrow> z = za"
+          foterm_to_hoterm z = (foterm_to_hoterm za :: ('\<tau>, 'c, 'f) preterm) \<Longrightarrow> z = za"
           using Fun\<^sub>s.IH by metis
       qed
 
@@ -134,14 +137,14 @@ proof (rule inj_onI)
   qed
 qed
 
-inductive eff_first_order where
-  Const: "eff_first_order (Const f)" |
+inductive eff_first_order :: "('\<tau>, 'c, 'f) preterm \<Rightarrow> bool" where
+  Const: "eff_first_order (Const f [] [])" |
   Free: "eff_first_order (Free x)" |
   App: "eff_first_order (App t\<^sub>1 t\<^sub>2)"
     if "eff_first_order t\<^sub>1" and "is_Const (head t\<^sub>1)" and "eff_first_order t\<^sub>2"
 
 lemma eff_first_orderE_foldl_App:
-  fixes t :: "('f, 'v) LN_HO_Term.term"
+  fixes t :: "('\<tau>, 'c, 'f) preterm"
   assumes "eff_first_order t"
   shows "is_Const t \<or> is_Free t \<or>
     (\<exists>xs. (\<forall>x \<in> set xs. eff_first_order x) \<and> t = foldl App (head t) xs)"
@@ -168,10 +171,10 @@ next
     assume "is_Free t\<^sub>1"
     hence False
       using App.hyps
-      by (metis head.simps(2) is_Free_def term.distinct_disc(1))
+      by (metis head.simps(2) is_Free_def preterm.distinct_disc(1))
     thus ?thesis ..
   next
-    fix xs :: "('f, 'v) LN_HO_Term.term list"
+    fix xs :: "('\<tau>, 'c, 'f) preterm list"
     assume "\<forall>x\<in>set xs. eff_first_order x" and "t\<^sub>1 = foldl App (head t\<^sub>1) xs"
     show ?thesis
     proof (intro exI conjI ballI)
@@ -189,8 +192,8 @@ next
 qed
 
 lemma App_eq_foldl_App_ConsD:
-  assumes "App t\<^sub>1 t\<^sub>2 = foldl App (Const f) xs"
-  shows "\<exists>xs'. xs = xs' @ [t\<^sub>2] \<and> t\<^sub>1 = foldl App (Const f) xs'"
+  assumes "App t\<^sub>1 t\<^sub>2 = foldl App (Const f [] []) xs"
+  shows "\<exists>xs'. xs = xs' @ [t\<^sub>2] \<and> t\<^sub>1 = foldl App (Const f [] []) xs'"
   using assms
   by (induction xs rule: List.rev_induct) simp_all
 
@@ -209,7 +212,8 @@ proof -
     case (Fun g ys)
     obtain y ys' where "ys = ys' @ [y]"
       using Fun.prems[simplified]
-      by (metis LN_HO_Term.term.distinct(5) foldl_Nil list.simps(8) rev_exhaust)
+      by (metis foldl_Nil list.simps(8) preterm.distinct(5) rev_exhaust)
+
     show ?case
       using Fun.prems[unfolded \<open>ys = ys' @ [y]\<close>, simplified]
       using Fun.IH
@@ -217,16 +221,19 @@ proof -
   qed
 qed
 
+lemma head_foldl_App[simp]: "head (foldl App x xs) = head x"
+  by (induction xs arbitrary: x rule: rev_induct) simp_all
+
 lemma
-  "bij_betw foterm_to_hoterm UNIV {t :: ('f, 'v) LN_HO_Term.term. eff_first_order t}"
+  "bij_betw foterm_to_hoterm UNIV {t :: ('\<tau>, 'c, 'f) preterm. eff_first_order t}"
   unfolding bij_betw_def
 proof (intro conjI)
   show "inj_on foterm_to_hoterm UNIV"
     using inj_on_foterm_to_hoterm .
 next
-  show "range foterm_to_hoterm = {t :: ('f, 'v) LN_HO_Term.term. eff_first_order t}"
+  show "range foterm_to_hoterm = {t :: ('\<tau>, 'c, 'f) preterm. eff_first_order t}"
   proof (intro subset_antisym subsetI , unfold mem_Collect_eq)
-    fix t :: "('f, 'v) LN_HO_Term.term"
+    fix t :: "('\<tau>, 'c, 'f) preterm"
     assume "t \<in> range foterm_to_hoterm"
     then obtain t\<^sub>G where "t = foterm_to_hoterm t\<^sub>G"
       by blast
@@ -238,19 +245,25 @@ next
         by (simp add: eff_first_order.Free)
     next
       case (Fun f xs)
-      hence "eff_first_order (foldl App (Const f) (map foterm_to_hoterm xs))"
+      hence "eff_first_order (foldl App (Const f [] []) (map foterm_to_hoterm xs :: ('\<tau>, 'c, 'f) preterm list))"
       proof (induction xs rule: List.rev_induct)
         case Nil
         then show ?case
         by (simp add: eff_first_order.Const)
       next
         case (snoc x xs)
-        have "eff_first_order (App (foldl App (Const f) (map foterm_to_hoterm xs))
+        have "eff_first_order (App (foldl App (Const f [] []) (map foterm_to_hoterm xs :: ('\<tau>, 'c, 'f) preterm list))
           (foterm_to_hoterm x))"
-        by (metis LN_HO_Term.term.disc(1) LN_HO_Term.term.simps(17) eff_first_order.cases
-            eff_first_order.intros(3) foterm_to_hoterm.simps(2)
-            foterm_to_hoterm_Fun_eq_Const_or_App head.simps(1,4) list.set_intros(1,2)
-            rotate1.simps(2) set_rotate1 snoc.IH snoc.prems)
+        proof (rule eff_first_order.App)
+          show "eff_first_order (foldl App (Const f [] []) (map foterm_to_hoterm xs :: ('\<tau>, 'c, 'f) preterm list))"
+            using snoc by simp
+        next
+          show "is_Const (head (foldl App (Const f [] []) (map foterm_to_hoterm xs :: ('\<tau>, 'c, 'f) preterm list)))"
+            by simp
+        next
+          show "eff_first_order (foterm_to_hoterm x :: ('\<tau>, 'c, 'f) preterm)"
+            by (simp add: snoc.prems)
+        qed
         thus ?case
           by simp
       qed
@@ -258,14 +271,14 @@ next
         by simp
     qed
   next
-    fix t :: "('f, 'v) LN_HO_Term.term"
+    fix t :: "('\<tau>, 'c, 'f) preterm"
     assume "eff_first_order t"
     thus "t \<in> range foterm_to_hoterm"
     proof (induction t rule: eff_first_order.induct)
       case (Const f)
       show ?case
       proof (rule range_eqI)
-        show "Const f = foterm_to_hoterm (Term.Fun f [])"
+        show "Const f [] [] = foterm_to_hoterm (Term.Fun f [])"
           by simp
       qed
     next
@@ -277,14 +290,19 @@ next
       qed
     next
       case (App t\<^sub>1 t\<^sub>2)
-      obtain f where "head t\<^sub>1 = Const f"
-        by (metis App.hyps(2) is_Const_def)
-      obtain xs where "(\<forall>x\<in>set xs. eff_first_order x)" and "App t\<^sub>1 t\<^sub>2 = foldl App (Const f) xs"
-        using eff_first_orderE_foldl_App[of "App t\<^sub>1 t\<^sub>2"] \<open>head t\<^sub>1 = Const f\<close>
+      obtain f :: 'c where "head t\<^sub>1 = Const f [] []"
+        by (metis (no_types, opaque_lifting) App.IH(1)
+            App.hyps(2) foterm_to_hoterm.simps(1,2)
+            head.simps(1,2) head_foldl_App preterm.disc(2)
+            rangeE vars_term_ms.cases)
+      obtain xs :: "('\<tau>, 'c, 'f) preterm list" where
+        "(\<forall>x\<in>set xs. eff_first_order x)" and "App t\<^sub>1 t\<^sub>2 = foldl App (Const f [] []) xs"
+        using eff_first_orderE_foldl_App[of "App t\<^sub>1 t\<^sub>2"] \<open>head t\<^sub>1 = Const f [] []\<close>
         by (auto simp: App.hyps(1,2,3) eff_first_order.App)
-      then obtain ys where "xs = ys @ [t\<^sub>2]" and "t\<^sub>1 = foldl App (Const f) ys"
+      then obtain ys :: "('\<tau>, 'c, 'f) preterm list" where
+        "xs = ys @ [t\<^sub>2]" and "t\<^sub>1 = foldl App (Const f [] []) ys"
         using App_eq_foldl_App_ConsD by metis
-      hence "foldl App (Const f) ys \<in> range foterm_to_hoterm"
+      hence "foldl App (Const f [] []) ys \<in> range foterm_to_hoterm"
         using App.IH(1) by simp
       hence "\<exists>ys\<^sub>G. ys = map foterm_to_hoterm ys\<^sub>G"
       proof (induction ys rule: List.rev_induct)
@@ -292,9 +310,11 @@ next
         then show ?case by simp
       next
         case (snoc x xs)
-        then have "App (foldl App (Const f) xs) x \<in> range foterm_to_hoterm"
+        then have "App (foldl App (Const f [] []) xs) x \<in> range foterm_to_hoterm"
           by simp
-        then have "foldl App (Const f) xs \<in> range foterm_to_hoterm" and "x \<in> range foterm_to_hoterm"
+        then have
+          "foldl App (Const f [] []) xs \<in> range foterm_to_hoterm" and
+          "x \<in> range foterm_to_hoterm"
           using App_in_range_fo_term_to_ho_termD by auto
         then show ?case
           using snoc.IH
@@ -318,7 +338,7 @@ next
       show ?case
       proof (rule range_eqI)
         show "App t\<^sub>1 t\<^sub>2 = foterm_to_hoterm (Term.Fun f xs\<^sub>G)"
-          unfolding \<open>App t\<^sub>1 t\<^sub>2 = foldl App (Const f) xs\<close>
+          unfolding \<open>App t\<^sub>1 t\<^sub>2 = foldl App (Const f [] []) xs\<close>
           by (simp add: \<open>xs = map foterm_to_hoterm xs\<^sub>G\<close>)
       qed
     qed
